Tigris/TCNF/interpreter/evalCEK.lean
@@ -1,0 +1,145 @@
+import Tigris.TCNF.interpreter.types
+import Tigris.TCNF.entrypoint
+namespace TCNF.Interpreter open Std TCNF open MLType (TypingError) open Array (seq2fold2)
+
+private def checkInterrupt : EIO TypingError Unit :=
+  IO.checkCanceled >>= fun
+  | true => throw .Interrupted
+  | false => return ()
+local macro "withInterrupt!" x:doSeq : term => ``(do $x)
+
+def computeLet (lv : LetValue .postCC) : EvaluatorCEK Value :=
+  match lv with
+  | .lit k         => return asConst k
+  | .pair p q      => .pair <$> evalAtom p <*> evalAtom q
+  | .proj i x      => projPair x i =<< lookup x
+  | .field _ i x   => projConstr x i =<< lookup x
+  | .ctor t as     => .constr t <$> as.mapM evalAtom
+  | .prim op args  => evalPrimBinop op =<< args.mapM evalAtom
+  | .extern f args => evalExtern f =<< args.mapM evalAtom
+  | .isCtor x t a =>
+    lookup x <&> fun
+    | .constr t' as => .bool (t' == t && as.size == a)
+    | _             => .bool false
+  | .mkClos c env => .clos c <$> env.mapM evalAtom
+  | _ => impossibleF! "computeLet: unexpected {format lv |>.pretty (indent := 23) (column := 23)}"
+
+mutual
+/-- evaluate the kontinuation stack. -/
+partial def «continue» (v : Value) (kont : Kont) : EvaluatorCEK Value := fun s =>
+  match kont with
+  | .halt => return v
+  | .letK fv rest env k =>
+    loop rest k {s with locals := env.insert fv v}
+  | .appK _ captured remaining k =>
+    match v with
+    | .clos c cap => applyCEK c (captured ++ cap) remaining k s
+    | _ => impossibleT! "over-application produced non-function {v}" kont $ s
+
+partial def applyCEK
+  (codeptr : FVarId)
+  (captured : Array Value)
+  (args : Subarray Value)
+  (kont : Kont) : EvaluatorCEK Value := fun s@{locals, globaldecls,..} =>
+  withInterrupt!
+    let some {params,body,..} := globaldecls[codeptr]? | impossibleT! "undefined function #{codeptr}" kont $ s
+    let arity  := params.size - captured.size
+    let ass    := args.size
+    if arity == ass then
+      let locals := seq2fold2 (fun acc a b => acc.insert b.fvarId a) locals captured args params
+      loop body kont {s with locals}
+    else if arity > ass then «continue» (.clos codeptr (captured ++ args)) kont s
+    else
+      let locals := seq2fold2 (fun acc a b => acc.insert b.fvarId a) locals captured args[:arity] params
+      loop body (.appK codeptr #[] args[arity:] kont) {s with locals}
+
+partial def evaluateLet (lv : LetValue .postCC) (kont : Kont) : EvaluatorCEK Value :=
+  match lv with
+  | .app 0 as | .pap 0 as =>
+    impossibleT! "All branches failed to match against {format as}" kont
+  | .app f as | .pap f as => withInterrupt!
+    let fv <- lookup f
+    let args <- as.mapM evalAtom
+    match fv with
+    | .clos c cap => applyCEK c cap args.toSubarray kont
+    | v => impossibleT! "callee {v} is not a code pointer" kont
+  | _ => do
+    let v <- computeLet lv
+    «continue» v kont
+
+partial def loop (code : Code .postCC) (kont : Kont) : EvaluatorCEK Value := fun s@{locals, joins,..} => withInterrupt!
+  match code with
+  | .let {fvarId, value,..} b =>
+    -- same tail-call peephole as in CL backend. here we skip the letK frame
+    let tail? := match b with
+      | .ret (.fvar r) => r == fvarId
+      | _              => false
+    let kont' := if tail? then kont else .letK fvarId b locals kont
+    evaluateLet value kont' s
+  | .ret a =>
+    let v <- evalAtom a s
+    «continue» v kont s
+  | .cases d _ alts =>
+    let v <- lookup d s
+    match v with
+    | .unit =>
+      match alts.find? fun | .default _ | .const .PUnit _ => true | _ => false
+      with | some (.default k) | some (.const _ k) => loop k kont s
+           | _ => impossibleT! "Can't match against {d} => ()" kont $ s
+    | .int i =>
+      match alts.find? fun | .default _ => true | .const (.PInt i') _ => i == i' | _ => false
+      with | some (.default k) | some (.const _ k) => loop k kont s
+           | _ => impossibleT! "Can't match against {d} => {i}" kont $ s
+    | .bool b =>
+      match alts.find? fun | .default _ => true | .const (.PBool b') _ => b == b' | _ => false
+      with | some (.default k) | some (.const _ k) => loop k kont s
+           | _ => impossibleT! "Can't match against {d} => {b}" kont $ s
+    | .str str =>
+      match alts.find? fun | .default _ => true | .const (.PStr s') _ => str == s' | _ => false
+      with | some (.default k) | some (.const _ k) => loop k kont s
+           | _ => impossibleT! "Can't match against {d} => {repr str}" kont $ s
+    | .constr t as =>
+      match alts.find? fun | .default _ => true | .ctor t' .. => t' == t | _ => false with
+      | some (.default k) => loop k kont s
+      | some (.ctor _ ps k) =>
+        let locals := Array.foldl2 (fun acc a {fvarId,..} => acc.insert fvarId a) locals as ps
+        loop k kont {s with locals}
+      | _ => impossibleT! "Can't match against {d} => {t}" kont $ s
+    | v => impossibleT! "Discriminant {v} is neither variant nor constant" kont $ s
+  | .jp {fvarId, params, body,..} k =>
+    let ps := params.map Param.fvarId
+    loop k kont {s with joins := joins.insert fvarId (ps, body, locals)}
+  | .jmp jp args => do
+    let some (ps, body, capturedEnv) := s.joins[jp]? | impossibleT! "undefined join point #{jp}" kont $ s
+    let as <- args.mapM evalAtom s
+    let locals := Array.foldl2 (fun acc fv a => acc.insert fv a) capturedEnv ps as
+    loop body kont {s with locals}
+  | .unreach _ => impossibleT! "unreachable code has been reached" kont $ s
+end
+open Format (fill group pretty nestD)
+def check (s : String) : LowerM Unit := do
+  let (_, topdecl) <- Parsing.parseModuleIR s initState
+  let stage₀@(_, E, _) <- inferToplevelC topdecl MLType.defaultE' |>.mapError toString |> EIO.ofExcept
+  let (fdecls, _, ctors) <- inferToplevelF stage₀ |>.mapError toString |> EIO.ofExcept
+  let {decls, main} <- lowerModuleCCOpt fdecls ctors E.tyDecl
+  let mut globaldecls := ∅
+  let mut topvals := ∅
+  for d@{fvarId, arity, body, name,..} in decls.push main do
+    if arity > 0 then
+      if let some ty := E.E[name]? then
+        liftEIO (println! template name "<fun>" ty)
+      globaldecls := globaldecls.insert fvarId d
+      topvals := topvals.insert fvarId (.clos fvarId #[])
+    else
+      let st : IState := {globaldecls, topvals, locals := ∅, joins := ∅}
+      let v <- loop body .halt |>.run st |>.adapt toString
+      if let some ty := E.E[name]? then
+        liftEIO (println! template name v ty)
+      topvals := topvals.insert fvarId v
+
+def checkFile (s : System.FilePath) : IO Unit := do
+  let s <- IO.FS.readFile s
+  EIO.toIO .userError $ check s
+
+def main (args : List String) :=
+  args.forA fun p => checkFile p
